more implementation of bb

theories/wz_bb.v
@@ -8,7 +8,30 @@ From Wasm Require Import datatypes list_extra.
 Import ListNotations.
 
 Local Open Scope bool_scope.
+(* 
+Inductive bb_instr_type :=
+  | BB_it_body
+  | BB_it_term.
 
+Definition bb_instr_type_of_bi (i: basic_instruction): bb_instr_type :=
+  match i with
+  | BI_unreachable
+  | BI_block _ _
+  | BI_loop _ _
+  | BI_if _ _ _
+  | BI_br _
+  | BI_br_if _
+  | BI_br_table _ _
+  | BI_return         => BB_it_term
+  | _                 => BB_it_body
+  end.
+
+Fixpoint is_bb_expr (is: list basic_instruction): bool :=
+  match is with
+  | [] => true
+  | x::xa => land (bb_instr_type_of_bi x) = BB_it_body
+  end.
+ *)  
 Inductive bb_t :=
   | BB_exit_end | BB_exit_return | BB_exit_unreachable
   | BB_block | BB_loop 
@@ -32,67 +55,55 @@ Definition bb_t_of_instr (i: basic_instruction): bb_t :=
   | _                 => BB_code
   end.
 
-(* This is the definition of bb from the OCaml code. It's only here for reference
-   and to allow some code that needs to be updated to continue to compile.
-   This definition will be deleted when we've completed the work on this module.
-*)
-Inductive bb : Type :=
+(* basic block - bb *)
+Record bb: Type :=
 {
-  bbindex:  nat;        (* the index of this bb in the list of bblocks, makes things easier to have this *)
-  start_op: nat;        (* index into e of the first op in the expr *)
-(*  mutable *) end_op:   nat;        (* index+1 of the last op in the expr *)
-(*  mutable *) succ:     list bb;    (* bblocks that can be directly reached from this bb *)
-(*  mutable *) pred:     list bb;    (* bblocks that can directly reach this bb *)
-(*  mutable *) bbtype:	 bb_t;       (* effectively the control opcode that created this bb *)
-(*  mutable *) nesting:  nat;        (* nesting level of the last opcode in the bb *)
-(*  mutable *) labels:   list nat;   (* destination labels used in BR, BR_IF, BR_TABLE instructions *)
-(*  mutable *) br_dest:	 option bb;  (* for LOOP, BLOCK and IF instructions the bb that's the target of a branch for this instruction  *)
-}.
-
-(* This is the new definition of bb' for the Rocq code *)
-Inductive bb': Type :=
-{
-  bb_index:   nat;
-  bb_type:    bb_t;
-  bb_nesting: nat;
-  bb_instrs:  list basic_instruction;
-  bb_succ:    list nat;
-  bb_pred:    list nat;
-  bb_br_dest: option nat;
+  bb_index:   nat;          (* the index of this bb in the list of bblocks *)
+  bb_instrs:  list basic_instruction; (* code of the bb *)
+  bb_type:    bb_t;         (* effectively the control opcode that created this bb *)
+  bb_nesting: nat;          (* nesting level of the last opcode in the bb *)
+  bb_labels:  list labelidx;(* destination labels used in BR, BR_IF, BR_TABLE instructions *)
+  bb_succ:    list nat;     (* bbs that can be directly reached from this bb *)
+  bb_pred:    list nat;     (* bbs that can directly reach this bb *)
+  bb_br_dest: option nat;   (* for LOOP, BLOCK and IF instructions the bb that's the target 
+                                of a branch for this instruction  *)
 }.
 
 Record bbs_progress: Type :=
 {
-    p_bb:       bb';
-    p_bbs:      list bb';
+    p_bb:       bb;
+    p_bbs:      list bb;
 }.
 
-Definition init_bb (idx: nat) (t: bb_t) (nesting: nat) (is: list basic_instruction): bb' :=
+Definition init_bb (idx: nat) (t: bb_t) (nesting: nat) (labels: list labelidx)
+             (is: list basic_instruction): bb :=
   {|  bb_index    := idx;
       bb_type     := t;
       bb_nesting  := nesting;
       bb_instrs   := is;
+      bb_labels   := labels;
       bb_succ     := []; 
       bb_pred     := [];
       bb_br_dest  := None |}.
 
-Definition bb_with_br_dest  (i: nat) (b: bb'): bb' :=
+Definition bb_with_br_dest  (i: nat) (b: bb): bb :=
   {|  bb_index    := bb_index b;
       bb_type     := bb_type b;
       bb_nesting  := bb_nesting b;
       bb_instrs   := bb_instrs b;
+      bb_labels   := bb_labels b;
       bb_succ     := bb_succ b; 
       bb_pred     := bb_pred b;
       bb_br_dest  := Some i |}.
   
 
-Definition empty_bb (idx: nat) (nesting: nat): bb' := init_bb idx BB_code nesting [].
+Definition empty_bb (idx: nat) (nesting: nat): bb := init_bb idx BB_code nesting [] [].
 
-(* bb's_pass1 determines bb_index, bb_type, bb_nesting, bb_instrs *)
-Fixpoint bb's_pass1 (bbs_prog: bbs_progress) (i: basic_instruction): bbs_progress :=
-  let bb's_pass1' (bbs_prog: bbs_progress) (e: expr): bbs_progress :=
+(* bbs_pass1 determines bb_index, bb_type, bb_nesting, bb_instrs *)
+Fixpoint bbs_pass1 (bbs_prog: bbs_progress) (i: basic_instruction): bbs_progress :=
+  let bbs_pass1' (bbs_prog: bbs_progress) (e: expr): bbs_progress :=
     
-    let bbs_prog' := List.fold_left bb's_pass1 e bbs_prog in
+    let bbs_prog' := List.fold_left bbs_pass1 e bbs_prog in
     let bb_acc    := (p_bb bbs_prog') in
     let bbs_acc   := (p_bbs bbs_prog') in
       (* did we wind up having a bb at the end?*)
@@ -101,67 +112,83 @@ Fixpoint bb's_pass1 (bbs_prog: bbs_progress) (i: basic_instruction): bbs_progres
       | [] => bbs_prog'
       (* yes, add it to the list of bbs *)
       | _ => {| p_bb  := empty_bb ((bb_index bb_acc)+1) (bb_nesting bb_acc);
-                p_bbs := ((init_bb (bb_index bb_acc) BB_code (bb_nesting bb_acc) (List.rev(bb_instrs bb_acc))))::bbs_acc |}
+                p_bbs := ((init_bb (bb_index bb_acc) BB_code (bb_nesting bb_acc) [] (List.rev(bb_instrs bb_acc))))::bbs_acc |}
       end
     in
     let bb_acc    := (p_bb  bbs_prog) in
     let bbs_acc   := (p_bbs bbs_prog) in
     match i with
       | BI_block b e1 =>
-          let e1_p := bb's_pass1' {| p_bb := empty_bb ((bb_index bb_acc)+1) ((bb_nesting (p_bb bbs_prog))+1);
+          let e1_p := bbs_pass1' {| p_bb := empty_bb ((bb_index bb_acc)+1) ((bb_nesting (p_bb bbs_prog))+1);
                                         p_bbs := [] |} e1 in
             {| p_bb   := empty_bb (bb_index (p_bb e1_p)) (bb_nesting bb_acc);
                p_bbs  := (p_bbs e1_p)
                           ++ (init_bb (bb_index bb_acc)
                                       BB_block
                                       (bb_nesting bb_acc)
+                                      []
                                       (List.rev ((BI_block b [])::(bb_instrs bb_acc))))::bbs_acc |}
       | BI_loop b e1 =>
-          let e1_p := bb's_pass1' {| p_bb := empty_bb((bb_index bb_acc)+1) ((bb_nesting (p_bb bbs_prog))+1);
+          let e1_p := bbs_pass1' {| p_bb := empty_bb((bb_index bb_acc)+1) ((bb_nesting (p_bb bbs_prog))+1);
                                         p_bbs := [] |} e1 in
             {| p_bb   := empty_bb (bb_index (p_bb e1_p)) (bb_nesting bb_acc);
                p_bbs  := (p_bbs e1_p)
                           ++ (init_bb (bb_index bb_acc)
                                       BB_loop
                                       (bb_nesting bb_acc)
+                                      []
                                       (List.rev ((BI_loop b [])::(bb_instrs bb_acc))))::bbs_acc |}
       | BI_if b e1 e2 =>
-          let e1_p := bb's_pass1' {| p_bb := empty_bb((bb_index bb_acc)+1) ((bb_nesting (p_bb bbs_prog))+1);
+          let e1_p := bbs_pass1' {| p_bb := empty_bb((bb_index bb_acc)+1) ((bb_nesting (p_bb bbs_prog))+1);
                                         p_bbs := [] |} e1 in
-          let e2_p := bb's_pass1' {| p_bb := empty_bb((bb_index (p_bb e1_p))+1) ((bb_nesting (p_bb e1_p))+1);
+          let e2_p := bbs_pass1' {| p_bb := empty_bb((bb_index (p_bb e1_p))+1) ((bb_nesting (p_bb e1_p))+1);
                                         p_bbs := []  |} e1 in
             {| p_bb   := (p_bb e2_p);
                p_bbs  := (p_bbs e2_p) ++ (p_bbs e2_p)
                           ++ (init_bb (bb_index (p_bb e2_p))
                                       BB_if
                                       (bb_nesting (p_bb e2_p))
+                                      []
                                       (List.rev ((BI_loop b [])::(bb_instrs bb_acc))))::bbs_acc |}
     | BI_unreachable
-    | BI_br _
-    | BI_br_if _
-    | BI_br_table _ _
     | BI_return =>
         {|  p_bb  := empty_bb ((bb_index bb_acc)+1) (bb_nesting (p_bb bbs_prog));
             p_bbs := (init_bb (bb_index bb_acc)
                               (bb_t_of_instr i)
                               (bb_nesting (p_bb bbs_prog))
+                              []
+                              (List.rev (i::(bb_instrs bb_acc))))::bbs_acc |}
+    | BI_br idx
+    | BI_br_if idx =>
+        {|  p_bb  := empty_bb ((bb_index bb_acc)+1) (bb_nesting (p_bb bbs_prog));
+            p_bbs := (init_bb (bb_index bb_acc)
+                              (bb_t_of_instr i)
+                              (bb_nesting (p_bb bbs_prog))
+                              [idx]
+                              (List.rev (i::(bb_instrs bb_acc))))::bbs_acc |}
+    | BI_br_table is _ =>
+        {|  p_bb  := empty_bb ((bb_index bb_acc)+1) (bb_nesting (p_bb bbs_prog));
+            p_bbs := (init_bb (bb_index bb_acc)
+                              (bb_t_of_instr i)
+                              (bb_nesting (p_bb bbs_prog))
+                              is
                               (List.rev (i::(bb_instrs bb_acc))))::bbs_acc |}
     | _ => 
-        {|  p_bb  := init_bb ((bb_index bb_acc)) BB_code (bb_nesting (p_bb bbs_prog)) (i::(bb_instrs bb_acc));
+        {|  p_bb  := init_bb ((bb_index bb_acc)) BB_code (bb_nesting (p_bb bbs_prog)) [] (i::(bb_instrs bb_acc));
             p_bbs := bbs_acc |}
   end.
 
-(* bb's_pass isn't really a pass, it adds the syntetic bbs to the list *)
-Definition bb's_pass2 (bbs: list bb'): list bb' :=
+(* bbs_pass2 isn't really a pass, it adds the synthetic bbs to the list *)
+Definition bbs_pass2 (bbs: list bb): list bb :=
   let i := List.length bbs in
-    bbs ++ [init_bb (i)   BB_exit_end         0 [];
-            init_bb (i+1) BB_exit_return      0 [];
-            init_bb (i+2) BB_exit_unreachable 0 []]
+    bbs ++ [init_bb (i)   BB_exit_end         0 [] [];
+            init_bb (i+1) BB_exit_return      0 [] [];
+            init_bb (i+2) BB_exit_unreachable 0 [] []]
   .
 
-(* bb's pass 3 determines bb_br_dest *)
-Definition bb's_pass3 (bbs: list bb'): list bb' :=
-  let bb's_pass3' (b: bb') :=
+(* bbs_pass3 determines bb_br_dest *)
+Definition bbs_pass3 (bbs: list bb): list bb :=
+  let bbs_pass3' (b: bb) :=
     match bb_type b with
     | BB_loop   => bb_with_br_dest ((bb_index b) + 1) b
     | BB_block 
@@ -175,10 +202,10 @@ Definition bb's_pass3 (bbs: list bb'): list bb' :=
     | _ => b
     end
     in
-  List.map bb's_pass3' bbs.
+  List.map bbs_pass3' bbs.
 
-(* bb's pass 4 determines the succ *)
-Definition bb's_pass4 (bbs: list bb'): list (list nat) :=
+(* bbs_pass_4 determines the succ *)
+Definition bbs_pass4 (bbs: list bb): list (list nat) :=
   let idx_of_else (idx: nat) (n: nat): option nat :=
     let bbs' := sublist idx (List.length bbs - idx) bbs in
       match find (fun b => (bb_nesting b) >= n) bbs' with
@@ -186,7 +213,7 @@ Definition bb's_pass4 (bbs: list bb'): list (list nat) :=
       | Some b => Some (bb_index b)
       end
   in
-  let succ_of_bb (idx: nat) (b: bb'): list nat :=
+  let succ_of_bb (idx: nat) (b: bb): list nat :=
     match bb_type b with
     | BB_exit_end
     | BB_exit_return
@@ -209,10 +236,10 @@ Definition bb's_pass4 (bbs: list bb'): list (list nat) :=
   in
   mapi succ_of_bb bbs.
 
-Definition bb's_of_expr (e: expr): list bb' :=
-  bb's_pass3 (
-  bb's_pass2 (
-  let p := List.fold_left bb's_pass1 e {| p_bb := empty_bb 0 0; p_bbs := [] |}
+Definition bbs_of_expr (e: expr): list bb :=
+  bbs_pass3 (
+  bbs_pass2 (
+  let p := List.fold_left bbs_pass1 e {| p_bb := empty_bb 0 0; p_bbs := [] |}
   in
     (* did we wind up having a bb at the end?*)
     match bb_instrs (p_bb p) with
@@ -222,16 +249,16 @@ Definition bb's_of_expr (e: expr): list bb' :=
     | _ => List.rev ((init_bb ((bb_index (p_bb p)))
                               BB_code
                               (bb_nesting (p_bb p))
+                              []
                               (List.rev (bb_instrs (p_bb p))))::(p_bbs p))
     end)).
 
 (* The simplest basic block *)
 Example simple_bb1 :
 forall (v1: value_num), 
-  bb's_of_expr [BI_const_num v1] 
-  = bb's_pass2 [(init_bb 0 BB_code 0 [BI_const_num v1])].
-Proof.
-  compute. reflexivity.
+  bbs_of_expr [BI_const_num v1] 
+  = bbs_pass2 [(init_bb 0 BB_code 0 [] [BI_const_num v1])].
+Proof. reflexivity.
 Qed.
 
 Definition i32_of n: i32 := Wasm_int.Int32.repr n.
@@ -239,31 +266,28 @@ Definition i32_of n: i32 := Wasm_int.Int32.repr n.
 (* A slightly more complicated example*)
 Example simple_bb2 :
 forall (v1: value_num) (v2: value_num), 
-  bb's_of_expr [BI_const_num v1; BI_const_num v2]
-  = bb's_pass2
-      [init_bb 0 BB_code 0 [BI_const_num v1; BI_const_num v2]].
-Proof.
-  reflexivity.
+  bbs_of_expr [BI_const_num v1; BI_const_num v2]
+  = bbs_pass2
+      [init_bb 0 BB_code 0 [] [BI_const_num v1; BI_const_num v2]].
+Proof. reflexivity.
 Qed.
 
 (* Now examples with instructions that terminate a bb *)
 Example branch_bb1 :
 forall v1 v2 v3 l, 
-  bb's_of_expr [BI_const_num v1; BI_const_num v2; BI_const_num v3; BI_br l]
-    = bb's_pass2
-      [init_bb 0 (BB_br l) 0 [BI_const_num v1; BI_const_num v2; BI_const_num v3; BI_br l]].
-Proof.
-  compute. reflexivity.
+  bbs_of_expr [BI_const_num v1; BI_const_num v2; BI_const_num v3; BI_br l]
+    = bbs_pass2
+      [init_bb 0 (BB_br l) 0 [l] [BI_const_num v1; BI_const_num v2; BI_const_num v3; BI_br l]].
+Proof. reflexivity.
 Qed.
 
 Example branch_bb2 :
 forall v1 v2 v3 l, 
-  bb's_of_expr [BI_const_num v1; BI_const_num v2; BI_br l; BI_const_num v3]
-  =   bb's_pass2
-      [ init_bb 0 (BB_br l) 0 [BI_const_num v1; BI_const_num v2; BI_br l];
-        init_bb 1 BB_code 0 [BI_const_num v3]].
-Proof.
-  compute. reflexivity.
+  bbs_of_expr [BI_const_num v1; BI_const_num v2; BI_br l; BI_const_num v3]
+  =   bbs_pass2
+      [ init_bb 0 (BB_br l) 0 [l] [BI_const_num v1; BI_const_num v2; BI_br l];
+        init_bb 1 BB_code 0 [] [BI_const_num v3]].
+Proof. reflexivity.
 Qed.
 
 Definition bubble_sort_expr: expr :=
@@ -349,15 +373,15 @@ Definition bubble_sort_expr: expr :=
     ]
 ].
 
-Compute bb's_pass4 (bb's_of_expr bubble_sort_expr).
+Compute bbs_pass4 (bbs_of_expr bubble_sort_expr).
 
-Definition bubble_sort_bbs: list bb' :=
-[ bb_with_br_dest 11 (init_bb 0 BB_block 0 [BI_block (BT_id 0%num) []]);
-  init_bb 1 (BB_br_if 0%num) 1 [BI_local_get 0%num;
+Definition bubble_sort_bbs: list bb :=
+[ bb_with_br_dest 11 (init_bb 0 BB_block 0 [] [BI_block (BT_id 0%num) []]);
+  init_bb 1 (BB_br_if 0%num) 1 [0%num] [BI_local_get 0%num;
           BI_const_num (VAL_int32 (i32_of 2));
           BI_relop T_i32 (Relop_i (ROI_lt SX_S));
           BI_br_if 0%num];
-  bb_with_br_dest 3 (init_bb 2 BB_loop 1 [BI_local_get 0%num;
+  bb_with_br_dest 3 (init_bb 2 BB_loop 1 [] [BI_local_get 0%num;
           BI_const_num (VAL_int32 (i32_of (-1)));
           BI_binop T_i32 (Binop_i BOI_add);
           BI_local_tee 2%num;
@@ -365,21 +389,21 @@ Definition bubble_sort_bbs: list bb' :=
           BI_const_num (VAL_int32 (i32_of 0));
           BI_local_set 4%num;
           BI_loop (BT_id 2%num) []]);
-  bb_with_br_dest 10 (init_bb 3 BB_block 2 [BI_local_get 3%num;
+  bb_with_br_dest 10 (init_bb 3 BB_block 2 [] [BI_local_get 3%num;
           BI_local_set 5%num;
           BI_const_num (VAL_int32 (i32_of 0));
           BI_local_set 6%num;
           BI_block (BT_id 0%num) []]);
-  init_bb 4 (BB_br_if 0%num) 3 [BI_local_get 4%num;
+  init_bb 4 (BB_br_if 0%num) 3 [0%num] [BI_local_get 4%num;
           BI_local_tee 7%num;
           BI_local_get 0%num;
           BI_binop T_i32 (Binop_i BOI_sub);
           BI_const_num (VAL_int32 (i32_of (-2)));
           BI_relop T_i32 (Relop_i (ROI_gt SX_S));
           BI_br_if 0%num];
-  bb_with_br_dest 6 (init_bb 5 BB_loop 3 [BI_loop (BT_id 4%num) []]);
-  bb_with_br_dest 9 (init_bb 6 BB_block 4 [BI_block (BT_id 0%num) []]);
-  init_bb 7 (BB_br_if 0%num) 5 [BI_local_get 1%num;
+  bb_with_br_dest 6 (init_bb 5 BB_loop 3 [] [BI_loop (BT_id 4%num) []]);
+  bb_with_br_dest 9 (init_bb 6 BB_block 4 [] [BI_block (BT_id 0%num) []]);
+  init_bb 7 (BB_br_if 0%num) 5 [0%num] [BI_local_get 1%num;
           BI_local_get 6%num;
           BI_local_tee 3%num;
           BI_const_num (VAL_int32 (i32_of 2));
@@ -401,19 +425,19 @@ Definition bubble_sort_bbs: list bb' :=
           BI_local_tee 9%num;
           BI_relop T_i32 (Relop_i (ROI_le SX_S));
           BI_br_if 0%num];
-  init_bb 8 BB_code 5 [BI_local_get 6%num;
+  init_bb 8 BB_code 5 [] [BI_local_get 6%num;
           BI_local_get 9%num;
           BI_store T_i32 None {| memarg_offset := 0%num;  memarg_align := 0%num |};
           BI_local_get 8%num;
           BI_local_get 4%num;
           BI_store T_i32 None {| memarg_offset := 0%num;  memarg_align := 0%num |}];
-  init_bb 9 (BB_br_if 0%num) 4 [BI_local_get 3%num;
+  init_bb 9 (BB_br_if 0%num) 4 [0%num] [BI_local_get 3%num;
           BI_local_set 6%num;
           BI_local_get 3%num;
           BI_local_get 5%num;
           BI_relop T_i32 (Relop_i ROI_ne);
           BI_br_if 0%num];
-  init_bb 10 (BB_br_if 0%num) 1 [BI_local_get 5%num;
+  init_bb 10 (BB_br_if 0%num) 1 [0%num] [BI_local_get 5%num;
           BI_const_num (VAL_int32 (i32_of (-1)));
           BI_binop T_i32 (Binop_i BOI_add);
           BI_local_set 3%num;
@@ -430,19 +454,18 @@ Definition bubble_sort_bbs: list bb' :=
 ].
 
 Compute List.length bubble_sort_bbs.
-Compute List.length (bb's_of_expr bubble_sort_expr).
+Compute List.length (bbs_of_expr bubble_sort_expr).
 Compute List.fold_left (fun a x => a + List.length (bb_instrs x)) bubble_sort_bbs 0.
-Compute List.fold_left (fun a x => a + List.length (bb_instrs x)) (bb's_of_expr bubble_sort_expr) 0.
+Compute List.fold_left (fun a x => a + List.length (bb_instrs x)) (bbs_of_expr bubble_sort_expr) 0.
 Compute List.map (fun x => List.length (bb_instrs x)) bubble_sort_bbs.
-Compute List.map (fun x => List.length (bb_instrs x)) (bb's_of_expr bubble_sort_expr).
+Compute List.map (fun x => List.length (bb_instrs x)) (bbs_of_expr bubble_sort_expr).
 Compute List.map (fun x => (bb_nesting x)) bubble_sort_bbs.
-Compute List.map (fun x => (bb_nesting x)) (bb's_of_expr bubble_sort_expr).
-Compute List.map (fun x => (bb_br_dest x)) (bb's_pass2 bubble_sort_bbs).
-Compute List.map (fun x => (bb_br_dest x)) (bb's_of_expr bubble_sort_expr).
+Compute List.map (fun x => (bb_nesting x)) (bbs_of_expr bubble_sort_expr).
+Compute List.map (fun x => (bb_br_dest x)) (bbs_pass2 bubble_sort_bbs).
+Compute List.map (fun x => (bb_br_dest x)) (bbs_of_expr bubble_sort_expr).
 
-Example bubble_sort: bb's_of_expr bubble_sort_expr = bb's_pass2 bubble_sort_bbs.
-Proof.
-  compute. reflexivity.
+Example bubble_sort: bbs_of_expr bubble_sort_expr = bbs_pass2 bubble_sort_bbs.
+Proof. reflexivity.
 Qed.
 
 Definition bb_instr: Type := option basic_instruction.
@@ -460,22 +483,8 @@ Definition bb_instr_of_basic_instruction (i: basic_instruction): bb_instr :=
     | _ => Some i
   end.
 
-Lemma bb_instr_not_block: forall (i: basic_instruction) (b: block_type) (e: expr),
-  bb_instr_of_basic_instruction i = Some i ->
-  i <> BI_block b e.
-Proof. intros i b e H. compute. intros E.
-Admitted.
-
-(*
-Lemma bb_of_instr: forall (i: basic_instruction),
-    bb_instr_of_basic_instruction i = Some i ->
-    bb's_of_expr ([i]) = [(init_bb ([i]))].
-Proof.
-Admitted.
-*)
-
 Definition bb_is_exit (b: bb): bool :=
-  match bbtype b with 
+  match bb_type b with 
     | BB_exit_end | BB_exit_return | BB_exit_unreachable => true 
     | _ => false
   end.
@@ -483,16 +492,15 @@ Definition bb_is_exit (b: bb): bool :=
 Definition non_exit_bbs (bblocks: list bb): list bb :=
   List.filter (fun bblock => (orb (bb_is_exit bblock) true)) bblocks.
 
-Definition cost_of_bb (b: bb): nat := 
-  (end_op b) - (start_op b).
+Definition cost_of_bb (b: bb): nat := List.length (bb_instrs b).
 
 Definition compare_bbs (b1: bb) (b2: bb): comparison :=
-  Nat.compare (bbindex b1) (bbindex b2).
+  Nat.compare (bb_index b1) (bb_index b2).
 
 Definition bb_in_bblocks (b: bb) (bbs: list bb): bool :=
   List.existsb 
     (fun b' =>
-      match (bbindex b) - (bbindex b') with |0 => true |_ => false
+      match (bb_index b) - (bb_index b') with |0 => true |_ => false
       end
     )
     bbs.
@@ -500,26 +508,17 @@ Definition bb_in_bblocks (b: bb) (bbs: list bb): bool :=
 Definition bb_not_in_bblocks (b: bb) (bbs: list bb): bool :=
   List.forallb
     (fun b' => 
-      match (bbindex b) - (bbindex b') with |0 => false |_ => true
+      match (bb_index b) - (bb_index b') with |0 => false |_ => true
       end
     )
     bbs.
     
 Definition indexes_of_bbs (bbs: list bb): list nat :=
-  List.map (fun x => (bbindex x)) bbs.
+  List.map (fun x => (bb_index x)) bbs.
 
 Definition mult_succ_count (bbs: list bb): nat :=
   List.fold_left
-    (fun a x => match (succ x) with |[] | [_] => a | _ => a+1 end)
+    (fun a x => match (bb_succ x) with |[] | [_] => a | _ => a+1 end)
     bbs 0.
 
-Definition bblocks_of_expr (_: expr): list bb :=
-[].
-
-Definition expr_of_bb (e: expr) (bblock: bb): expr :=
-  sublist (start_op bblock) ((end_op bblock) - (start_op bblock)) e.
-
-(* 
-val expr_of_bb        : Wm.expr -> bb -> Wm.expr
-val bblocks_of_expr   : Wm.expr -> bb list
-*)
+Definition expr_of_bb (b: bb): expr := bb_instrs b.
